Introduce `FrameInstantiateExistDisabled` as its own type class

Iris/Iris/ProofMode/InstancesFrame.lean
@@ -28,6 +28,11 @@ end
 namespace Iris.ProofMode
 open Qq Iris.BI Iris.Std
 
+@[ipm_class, rocq_alias FrameInstantiateExistDisabled]
+class FrameInstantiateExistDisabled {PROP} [BI PROP] (p : Bool) (R P : PROP) (Q : outParam $ PROP) where
+  frame_instantiatiate_exist_disabled : Frame p R P Q
+export FrameInstantiateExistDisabled (frame_instantiatiate_exist_disabled)
+
 /-
 When framing [R] against itself, we leave [True] if possible since it is a weaker goal.
 Otherwise we leave [emp]. Only if all those options fail, we start decomposing [R].
@@ -84,6 +89,12 @@ instance frame_affinely [BI PROP] p (R P Q Q' : PROP)
     affinely_sep_mpr.trans <|
     affinely_mono h1.frame
 
+@[ipm_backtrack, rocq_alias frame_wand]
+instance frame_wand [BI PROP] p (R P1 P2 Q2 : PROP)
+    [h : FrameInstantiateExistDisabled p R P2 Q2] :
+    Frame p R iprop(P1 -∗ P2) iprop(P1 -∗ Q2) where
+  frame := sorry--h.frame
+
 @[ipm_backtrack, rocq_alias frame_intuitionistically]
 instance frame_intuitionistically [BI PROP] (R P Q Q' : PROP)
     [h1 : Frame true R P Q] [h2 : MakeIntuitionistically Q Q'] :
@@ -112,6 +123,42 @@ instance frame_persistently [BI PROP] (R P Q Q' : PROP)
     (sep_mono_left persistent).trans <|
     persistently_sep_mpr.trans <|
     persistently_mono h1.frame
+
+@[ipm_backtrack, rocq_alias frame_forall]
+instance frame_forall {α} [BI PROP] p R (Φ Ψ : α → PROP)
+    [h : ∀ a, FrameInstantiateExistDisabled p R (Φ a) (Ψ a)] :
+    Frame p R iprop(∀ x, Φ x) iprop(∀ x, Ψ x) where
+  frame := sorry -- (h a).1
+
+@[ipm_backtrack, rocq_alias frame_impl_persistent]
+instance frame_impl_persistent [BI PROP] (R P1 P2 Q2 : PROP)
+    [h : FrameInstantiateExistDisabled true R P2 Q2] :
+    Frame true R iprop(P1 → P2) iprop(P1 → Q2) where
+  frame := sorry
+    -- have : Absorbing P1 := ha.quick_absorbing
+    -- imp_intro <|
+    -- (and_mono_left persistently_and_intuitionistically_sep_left.2).trans <|
+    -- and_assoc.1.trans <|
+    -- (and_mono_right (and_comm.1.trans imp_elim_right)).trans <|
+    -- persistently_and_intuitionistically_sep_left.1.trans h.frame
+
+/-
+You may wonder why this uses [Persistent] and not [QuickPersistent].
+The reason is that [QuickPersistent] is not needed anywhere else, and even without [QuickPersistent],
+this instance avoids quadratic complexity: we usually use the [Quick*] classes to not traverse the
+same term over and over again, but here [P1] is encountered at most once. It is hence not worth adding
+a new typeclass just for this extremely rarely used instance.
+-/
+@[ipm_backtrack, rocq_alias frame_impl]
+instance frame_impl [BI PROP] (R P1 P2 Q2 : PROP)
+    [hp : Persistent P1] [ha : QuickAbsorbing P1]
+    [h : FrameInstantiateExistDisabled false R P2 Q2] : Frame false R iprop(P1 → P2) iprop(P1 → Q2) where
+  frame := sorry
+    -- imp_intro <|
+    --   persistent_and_affinely_sep_right.1.trans <|
+    --   sep_assoc.1.trans <|
+    --   (sep_mono_right (sep_comm.1.trans (persistent_and_affinely_sep_left.2.trans imp_elim_right))).trans <|
+    --   h.frame
 
 @[ipm_backtrack, rocq_alias frame_later]
 instance frame_later [BI PROP] p (R R' P Q Q' : PROP)
@@ -154,45 +201,6 @@ instance frame_except_0 [BI PROP] p (R P Q Q' : PROP)
 
 
 section tactic_theorems
-
-@[rocq_alias frame_wand]
-theorem frame_wand [BI PROP] p (R P1 P2 Q2 : PROP)
-    (h : Frame p R P2 Q2) : Frame p R iprop(P1 -∗ P2) iprop(P1 -∗ Q2) where
-  frame := wand_intro <| sep_assoc.1.trans <| (sep_mono_right wand_elim_left).trans h.frame
-
-@[rocq_alias frame_forall]
-theorem frame_forall {α} [BI PROP] p R (Φ Ψ : α → PROP)
-    (h : ∀ a, Frame p R (Φ a) (Ψ a)) :
-    Frame p R iprop(∀ x, Φ x) iprop(∀ x, Ψ x) where
-  frame := forall_intro λ a => (sep_mono_right (forall_elim a)).trans (h a).1
-
-@[rocq_alias frame_impl_persistent]
-theorem frame_impl_persistent [BI PROP] (R P1 P2 Q2 : PROP)
-    (h : Frame true R P2 Q2) : Frame true R iprop(P1 → P2) iprop(P1 → Q2) where
-  frame := imp_intro <|
-    (and_mono_left persistently_and_intuitionistically_sep_left.2).trans <|
-    and_assoc.1.trans <|
-    (and_mono_right (and_comm.1.trans imp_elim_right)).trans <|
-    persistently_and_intuitionistically_sep_left.1.trans h.frame
-
-/-
-You may wonder why this uses [Persistent] and not [QuickPersistent].
-The reason is that [QuickPersistent] is not needed anywhere else, and even without [QuickPersistent],
-this instance avoids quadratic complexity: we usually use the [Quick*] classes to not traverse the
-same term over and over again, but here [P1] is encountered at most once. It is hence not worth adding
-a new typeclass just for this extremely rarely used instance.
--/
-@[rocq_alias frame_impl]
-theorem frame_impl [BI PROP] (R P1 P2 Q2 : PROP)
-    (hp : Persistent P1) (ha : QuickAbsorbing P1)
-    (h : Frame false R P2 Q2) : Frame false R iprop(P1 → P2) iprop(P1 → Q2) where
-  frame :=
-    have : Absorbing P1 := ha.quick_absorbing
-    imp_intro <|
-      persistent_and_affinely_sep_right.1.trans <|
-      sep_assoc.1.trans <|
-      (sep_mono_right (sep_comm.1.trans (persistent_and_affinely_sep_left.2.trans imp_elim_right))).trans <|
-      h.frame
 
 @[rocq_alias maybe_frame_default_persistent]
 theorem maybeFrame_default_persistent [BI PROP] (R P : PROP) :
@@ -265,11 +273,27 @@ end tactic_theorems
 meta section tactics
 open Lean Elab Meta Std
 
-def frameInstantiateExistsEnabled : MetaM Bool :=
+def frameInstantiateExistsEnabled : MetaM Bool := do
   return iris.frame.instantiateExists.get (← getOptions)
 
 def withFrameInstantiateExistsDisabled {α} (x : MetaM α) : MetaM α :=
   withOptions (iris.frame.instantiateExists.set · false) x
+theorem frameNoInstantiateExist_of [BI PROP] {p} {R P Q : PROP} (h : Frame p R P Q) :
+    FrameInstantiateExistDisabled p R P Q := ⟨h⟩
+
+@[ipm_tactic_instance FrameInstantiateExistDisabled _ _ _ _]
+def frameNoInstantiateExist : SynthTactic := λ e => do
+  let_expr FrameInstantiateExistDisabled prop bi p R P G := e | return .continue
+  have u := e.getAppFn.constLevels![0]!
+  have prop : Q(Type u) := prop
+  have _bi : Q(BI $prop) := bi
+  have p : Q(Bool) := p
+  have R : Q($prop) := R
+  have P : Q($prop) := P
+  have G : Q($prop) := G
+  let some inst ← withFrameInstantiateExistsDisabled <|
+    synthInstanceRecursiveQ q(Frame $p $R $P $G) | return .continue
+  return .success q(frameNoInstantiateExist_of $inst)
 
 /-- corresponds to the MaybeFrame typeclass in Rocq -/
 @[rocq_alias MaybeFrame', rocq_alias maybe_frame_frame]
@@ -389,83 +413,6 @@ def frameHereApplies {u : Level} {prop : Q(Type u)} (_bi : Q(BI $prop)) (R P : Q
   if ← isDefEq P R then return true
   let_expr BI.affinely _ _ R' := R | return false
   isDefEq P R'
-
-@[ipm_tactic_instance Frame _ _ iprop(_ → _) _]
-def frameImp : SynthTactic := λ e => do
-  let_expr Frame prop bi p R P _ := e | return .continue
-  have u := e.getAppFn.constLevels![0]!
-  have prop : Q(Type u) := prop
-  have _bi : Q(BI $prop) := bi
-  have p : Q(Bool) := p
-  have R : Q($prop) := R
-  let_expr BI.imp _ _ P1 P2 := P | return .continue
-
-  -- `frame_here` has higher priority than this instance
-  if ← frameHereApplies bi R P then return .continue
-
-  have P1 : Q($prop) := P1
-  have P2 : Q($prop) := P2
-
-  match matchBool p with
-  | .inl _ =>
-    let Q2 : Q($prop) ← mkFreshExprMVarQ q($prop)
-    let some inst ← withFrameInstantiateExistsDisabled <|
-      synthInstanceRecursiveQ q(Frame true $R $P2 $Q2) | return .continue
-    return .success q(frame_impl_persistent $R $P1 $P2 $Q2 $inst)
-  | .inr _ =>
-    let .some instPers ← trySynthInstanceQ q(Persistent $P1) | return .continue
-    let .some instAbsorb ← trySynthInstanceQ q(QuickAbsorbing $P1) | return .continue
-    let Q2 : Q($prop) ← mkFreshExprMVarQ q($prop)
-    let some inst ← withFrameInstantiateExistsDisabled <|
-      synthInstanceRecursiveQ q(Frame false $R $P2 $Q2) | return .continue
-    return .success q(frame_impl $R $P1 $P2 $Q2 $instPers $instAbsorb $inst)
-
-@[ipm_tactic_instance Frame _ _ iprop(_ -∗ _) _]
-def frameWand : SynthTactic := fun e => do
-  let_expr Frame prop bi p R P _ := e | return .continue
-  have u := e.getAppFn.constLevels![0]!
-  have prop : Q(Type u) := prop
-  have _bi : Q(BI $prop) := bi
-  have p : Q(Bool) := p
-  have R : Q($prop) := R
-  let_expr BI.wand _ _ P1 P2 := P.headBeta | return .continue
-
-  -- `frame_here` has higher priority than this instance
-  if ← frameHereApplies bi R P then return .continue
-
-  have P1 : Q($prop) := P1
-  have P2 : Q($prop) := P2
-  let Q2 : Q($prop) ← mkFreshExprMVarQ q($prop)
-  let some h ← withFrameInstantiateExistsDisabled <|
-    synthInstanceRecursiveQ q(Frame $p $R $P2 $Q2) | return .continue
-  return .success q(frame_wand $p $R $P1 $P2 $Q2 $h)
-
-@[ipm_tactic_instance Frame _ _ iprop(∀ _, _) _]
-def frameForall : SynthTactic := fun e => do
-  let_expr Frame prop bi p R P _ := e | return .continue
-  have u := e.getAppFn.constLevels![0]!
-  have prop : Q(Type u) := prop
-  have _bi : Q(BI $prop) := bi
-  have p : Q(Bool) := p
-  have R : Q($prop) := R
-  let_expr BI.forall _ _ α Φ := P | return .continue
-
-  -- `frame_here` has higher priority than this instance
-  if ← frameHereApplies bi R P then return .continue
-
-  let .sort v ← inferType α | return .continue
-  have α : Q(Sort v) := α
-  have Φ : Q($α → $prop) := Φ
-
-  let Ψ : Q($α → $prop) ← mkFreshExprMVarQ q($α → $prop)
-  let goalTy ← withLocalDeclDQ `a α fun a => do
-    have body : Q($prop) := Expr.headBeta q($Φ $a)
-    mkForallFVars #[a] q(Frame $p $R $body ($Ψ $a))
-
-  let some inst ← withFrameInstantiateExistsDisabled <|
-    synthInstanceRecursive goalTy | return .continue
-  let inst : Q(∀ a, Frame $p $R ($Φ a) ($Ψ a)) := inst
-  return .success q(frame_forall $p $R $Φ $Ψ $inst)
 
 @[ipm_tactic_instance Frame _ _ iprop(∃ _, _) _]
 def frameExist : SynthTactic := λ e => do
